Verify fe25519_sq.

fe25519/fe25519_sq.v
@@ -1,6 +1,9 @@
 From Coq Require Import ZArith .
-From mQhasm Require Import mQhasm .
+From mQhasm Require Import mQhasm Radix .
 From mathcomp Require Import seq .
+
+Open Scope N_scope.
+Open Scope mqhasm_scope.
 
 Definition fe25519_sq : program :=
 let         wsize :=   64%positive in
@@ -53,10 +56,6 @@ let           tmp := 998 in
 let         carry := 999 in
 
 [::
-      (* # CPU: Intel(R) Xeon(R) CPU X5675 @ 3.07GHz *)
-      (* # RAM: 32GB *)
-      (* # Configuration: -c consts -s *)
-      (* # With Boolector 1.6.0 (-minisat): ? *)
       (*  *)
       (* int64 rp *)
       (* int64 xp *)
@@ -121,23 +120,6 @@ let         carry := 999 in
       (* c6_stack = c6 *)
       (* c7_stack = c7 *)
       (*  *)
-      (* ################################################################### *)
-      (* # Conditions on the inputs: x0 = *[uint64 *](xp +  0), *)
-      (* #                           x1 = *[uint64 *](xp +  8), *)
-      (* #                           x2 = *[uint64 *](xp + 16), *)
-      (* #                           x3 = *[uint64 *](xp + 24), *)
-      (* #                           x4 = *[uint64 *](xp + 32), are all in [0,2^54-1] *)
-      (* # *)
-      (* ################################################################### *)
-      (*  *)
-      (*   #// var x0 = mem64[xp + 0]@u520 *)
-      (*   #//     x1 = mem64[xp + 8]@u520 *)
-      (*   #//     x2 = mem64[xp + 16]@u520 *)
-      (*   #//     x3 = mem64[xp + 24]@u520 *)
-      (*   #//     x4 = mem64[xp + 32]@u520 *)
-      (*  *)
-      (*   #// assume 0 <=u x0, x1, x2, x3, x4 <u 2**54 *)
-      (*  *)
       (*   #BEGIN MACRO  *)
       (*   rax = *[uint64 *](xp + 0) *)
       (*   (uint128) rdx rax = rax * *[uint64 *](xp + 0) *)
@@ -158,301 +140,240 @@ QSplit rdx rax (QBinop QMul (QVar rax) (QVar x1)) wsize;
 QAssign r1 (QVar rax);
 QAssign r11 (QVar rdx);
       (*   rax = *[uint64 *](xp + 0) *)
-QAssign rax (QVar x0);
       (*   rax <<= 1 *)
-QAssign rax (QBinop QMul (QVar rax) qtwo);
       (*   (uint128) rdx rax = rax * *[uint64 *](xp + 16) *)
-QSplit rdx rax (QBinop QMul (QVar rax) (QVar x2)) wsize;
       (*   r2 = rax *)
-QAssign r2 (QVar rax);
       (*   r21 = rdx *)
+QAssign rax (QVar x0);
+QAssign rax (QBinop QMul (QVar rax) qtwo);
+QSplit rdx rax (QBinop QMul (QVar rax) (QVar x2)) wsize;
+QAssign r2 (QVar rax);
 QAssign r21 (QVar rdx);
       (*   rax = *[uint64 *](xp + 0) *)
-QAssign rax (QVar x0);
       (*   rax <<= 1 *)
-QAssign rax (QBinop QMul (QVar rax) qtwo);
       (*   (uint128) rdx rax = rax * *[uint64 *](xp + 24) *)
-QSplit rdx rax (QBinop QMul (QVar rax) (QVar x3)) wsize;
       (*   r3 = rax *)
-QAssign r3 (QVar rax);
       (*   r31 = rdx *)
+QAssign rax (QVar x0);
+QAssign rax (QBinop QMul (QVar rax) qtwo);
+QSplit rdx rax (QBinop QMul (QVar rax) (QVar x3)) wsize;
+QAssign r3 (QVar rax);
 QAssign r31 (QVar rdx);
       (*   rax = *[uint64 *](xp + 0) *)
-QAssign rax (QVar x1);
       (*   rax <<= 1 *)
-QAssign rax (QBinop QMul (QVar rax) qtwo);
       (*   (uint128) rdx rax = rax * *[uint64 *](xp + 32) *)
-QSplit rdx rax (QBinop QMul (QVar rax) (QVar x4)) wsize;
       (*   r4 = rax *)
-QAssign r4 (QVar rax);
       (*   r41 = rdx *)
+QAssign rax (QVar x0);
+QAssign rax (QBinop QMul (QVar rax) qtwo);
+QSplit rdx rax (QBinop QMul (QVar rax) (QVar x4)) wsize;
+QAssign r4 (QVar rax);
 QAssign r41 (QVar rdx);
       (*  *)
       (*   rax = *[uint64 *](xp + 8) *)
-QAssign rax (QVar x1);
       (*   (uint128) rdx rax = rax * *[uint64 *](xp + 8) *)
-QSplit rdx rax (QBinop QMul (QVar rax) (QVar x1)) wsize;
       (*   carry? r2 += rax *)
+      (*   r21 += rdx + carry *)
+QAssign rax (QVar x1);
+QSplit rdx rax (QBinop QMul (QVar rax) (QVar x1)) wsize;
 QAssign r2 (QBinop QAdd (QVar r2) (QVar rax));
 QSplit carry r2 (QVar r2) wsize;
-      (*   r21 += rdx + carry *)
 QAssign r21 (QBinop QAdd (QVar r21) (QBinop QAdd (QVar rdx) (QVar carry)));
       (*   rax = *[uint64 *](xp + 8) *)
-QAssign rax (QVar x1);
       (*   rax <<= 1 *)
-QAssign rax (QBinop QMul (QVar rax) qtwo);
       (*   (uint128) rdx rax = rax * *[uint64 *](xp + 16) *)
-QSplit rdx rax (QBinop QMul (QVar rax) (QVar x2)) wsize;
       (*   carry? r3 += rax *)
+      (*   r31 += rdx + carry *)
+QAssign rax (QVar x1);
+QAssign rax (QBinop QMul (QVar rax) qtwo);
+QSplit rdx rax (QBinop QMul (QVar rax) (QVar x2)) wsize;
 QAssign r3 (QBinop QAdd (QVar r3) (QVar rax));
 QSplit carry r3 (QVar r3) wsize;
-      (*   r31 += rdx + carry *)
 QAssign r31 (QBinop QAdd (QVar r31) (QBinop QAdd (QVar rdx) (QVar carry)));
       (*   rax = *[uint64 *](xp + 8) *)
-QAssign rax (QVar x1);
       (*   rax <<= 1 *)
-QAssign rax (QBinop QMul (QVar rax) qtwo);
       (*   (uint128) rdx rax = rax * *[uint64 *](xp + 24) *)
-QSplit rdx rax (QBinop QMul (QVar rax) (QVar x3)) wsize;
       (*   carry? r4 += rax *)
+      (*   r41 += rdx + carry *)
+QAssign rax (QVar x1);
+QAssign rax (QBinop QMul (QVar rax) qtwo);
+QSplit rdx rax (QBinop QMul (QVar rax) (QVar x3)) wsize;
 QAssign r4 (QBinop QAdd (QVar r4) (QVar rax));
 QSplit carry r4 (QVar r4) wsize;
-      (*   r41 += rdx + carry *)
 QAssign r41 (QBinop QAdd (QVar r41) (QBinop QAdd (QVar rdx) (QVar carry)));
       (*   rax = *[uint64 *](xp + 8) *)
-QAssign rax (QVar x1);
       (*   rax *= 38 *)
-QAssign rax (QBinop QMul (QVar rax) (QConst 38%Z));
       (*   (uint128) rdx rax = rax * *[uint64 *](xp + 32) *)
-QSplit rdx rax (QBinop QMul (QVar rax) (QVar x4)) wsize;
       (*   carry? r0 += rax *)
+      (*   r01 += rdx + carry *)
+QAssign rax (QVar x1);
+QAssign rax (QBinop QMul (QVar rax) (QConst 38%Z));
+QSplit rdx rax (QBinop QMul (QVar rax) (QVar x4)) wsize;
 QAssign r0 (QBinop QAdd (QVar r0) (QVar rax));
 QSplit carry r0 (QVar r0) wsize;
-      (*   r01 += rdx + carry *)
 QAssign r01 (QBinop QAdd (QVar r01) (QBinop QAdd (QVar rdx) (QVar carry)));
       (*    *)
       (*   rax = *[uint64 *](xp + 16) *)
-QAssign rax (QVar x2);
       (*   (uint128) rdx rax = rax * *[uint64 *](xp + 16) *)
-QSplit rdx rax (QBinop QMul (QVar rax) (QVar x2)) wsize;
       (*   carry? r4 += rax *)
+      (*   r41 += rdx + carry *)
+QAssign rax (QVar x2);
+QSplit rdx rax (QBinop QMul (QVar rax) (QVar x2)) wsize;
 QAssign r4 (QBinop QAdd (QVar r4) (QVar rax));
 QSplit carry r4 (QVar r4) wsize;
-      (*   r41 += rdx + carry *)
 QAssign r41 (QBinop QAdd (QVar r41) (QBinop QAdd (QVar rdx) (QVar carry)));
       (*   rax = *[uint64 *](xp + 16) *)
-QAssign rax (QVar x2);
       (*   rax *= 38 *)
-QAssign rax (QBinop QMul (QVar rax) (QConst 38%Z));
       (*   (uint128) rdx rax = rax * *[uint64 *](xp + 24) *)
-QSplit rdx rax (QBinop QMul (QVar rax) (QVar x3)) wsize;
       (*   carry? r0 += rax *)
+      (*   r01 += rdx + carry *)
+QAssign rax (QVar x2);
+QAssign rax (QBinop QMul (QVar rax) (QConst 38%Z));
+QSplit rdx rax (QBinop QMul (QVar rax) (QVar x3)) wsize;
 QAssign r0 (QBinop QAdd (QVar r0) (QVar rax));
 QSplit carry r0 (QVar r0) wsize;
-      (*   r01 += rdx + carry *)
 QAssign r01 (QBinop QAdd (QVar r01) (QBinop QAdd (QVar rdx) (QVar carry)));
       (*   rax = *[uint64 *](xp + 16) *)
-QAssign rax (QVar x2);
       (*   rax *= 38 *)
-QAssign rax (QBinop QMul (QVar rax) (QConst 38%Z));
       (*   (uint128) rdx rax = rax * *[uint64 *](xp + 32) *)
-QSplit rdx rax (QBinop QMul (QVar rax) (QVar x4)) wsize;
       (*   carry? r1 += rax *)
+      (*   r11 += rdx + carry *)
+QAssign rax (QVar x2);
+QAssign rax (QBinop QMul (QVar rax) (QConst 38%Z));
+QSplit rdx rax (QBinop QMul (QVar rax) (QVar x4)) wsize;
 QAssign r1 (QBinop QAdd (QVar r1) (QVar rax));
 QSplit carry r1 (QVar r1) wsize;
-      (*   r11 += rdx + carry *)
 QAssign r11 (QBinop QAdd (QVar r11) (QBinop QAdd (QVar rdx) (QVar carry)));
       (*    *)
       (*   rax = *[uint64 *](xp + 24) *)
-QAssign rax (QVar x3);
       (*   rax *= 19 *)
-QAssign rax (QBinop QMul (QVar rax) (QConst 19%Z));
       (*   (uint128) rdx rax = rax * *[uint64 *](xp + 24) *)
-QSplit rdx rax (QBinop QMul (QVar rax) (QVar x3)) wsize;
       (*   carry? r1 += rax *)
+      (*   r11 += rdx + carry *)
+QAssign rax (QVar x3);
+QAssign rax (QBinop QMul (QVar rax) (QConst 19%Z));
+QSplit rdx rax (QBinop QMul (QVar rax) (QVar x3)) wsize;
 QAssign r1 (QBinop QAdd (QVar r1) (QVar rax));
 QSplit carry r1 (QVar r1) wsize;
-      (*   r11 += rdx + carry *)
 QAssign r11 (QBinop QAdd (QVar r11) (QBinop QAdd (QVar rdx) (QVar carry)));
       (*   rax = *[uint64 *](xp + 24) *)
-QAssign rax (QVar x3);
       (*   rax *= 38 *)
-QAssign rax (QBinop QMul (QVar rax) (QConst 38%Z));
       (*   (uint128) rdx rax = rax * *[uint64 *](xp + 32) *)
-QSplit rdx rax (QBinop QMul (QVar rax) (QVar x4)) wsize;
       (*   carry? r2 += rax *)
+      (*   r21 += rdx + carry *)
+QAssign rax (QVar x3);
+QAssign rax (QBinop QMul (QVar rax) (QConst 38%Z));
+QSplit rdx rax (QBinop QMul (QVar rax) (QVar x4)) wsize;
 QAssign r2 (QBinop QAdd (QVar r2) (QVar rax));
 QSplit carry r2 (QVar r2) wsize;
-      (*   r21 += rdx + carry *)
 QAssign r21 (QBinop QAdd (QVar r21) (QBinop QAdd (QVar rdx) (QVar carry)));
       (*    *)
       (*   rax = *[uint64 *](xp + 32) *)
-QAssign rax (QVar x4);
       (*   rax *= 19 *)
-QAssign rax (QBinop QMul (QVar rax) (QConst 19%Z));
       (*   (uint128) rdx rax = rax * *[uint64 *](xp + 32) *)
-QSplit rdx rax (QBinop QMul (QVar rax) (QVar x4)) wsize;
       (*   carry? r3 += rax *)
+      (*   r31 += rdx + carry *)
+QAssign rax (QVar x4);
+QAssign rax (QBinop QMul (QVar rax) (QConst 19%Z));
+QSplit rdx rax (QBinop QMul (QVar rax) (QVar x4)) wsize;
 QAssign r3 (QBinop QAdd (QVar r3) (QVar rax));
 QSplit carry r3 (QVar r3) wsize;
-      (*   r31 += rdx + carry *)
 QAssign r31 (QBinop QAdd (QVar r31) (QBinop QAdd (QVar rdx) (QVar carry)));
       (*  *)
-      (*   #     lhs_520 = (x0 + x1 * 2**51 + x2 * 2**102 + x3 * 2**153 + x4 * 2**204) * (x0 + x1 * 2**51 + x2 * 2**102 + x3 * 2**153 + x4 * 2**204) *)
       (*  *)
-      (*   #// var r0_520 = (r01@u128.r0@u128)@u520 *)
-      (*   #//     r1_520 = (r11@u128.r1@u128)@u520 *)
-      (*   #//     r2_520 = (r21@u128.r2@u128)@u520 *)
-      (*   #//     r3_520 = (r31@u128.r3@u128)@u520 *)
-      (*   #//     r4_520 = (r41@u128.r4@u128)@u520 *)
-      (*   #//     lhs_520 = x0 * x0 + (2 * x0 * x1) * 2**51 + (2 * x0 * x2 + x1 * x1) * 2**102 + (2 * x0 * x3 + 2 * x1 * x2) * 2**153 + *)
-      (*   #//               (2 * x0 * x4 + 2 * x1 * x3 + x2 * x2) * 2**204 + (2 * x1 * x4 + 2 * x2 * x3) * 2**255 + (2 * x2 * x4 + x3 * x3) * 2**306 + *)
-      (*   #//               (2 * x3 * x4) * 2**357 + (x4 * x4) * 2**408 *)
-      (*   #//     rhs_520 = r0_520 + r1_520 * 2**51 + r2_520 * 2**102 + r3_520 * 2**153 + r4_520 * 2**204 *)
-      (*   #// assert lhs_520 >=u rhs_520 && (lhs_520 - rhs_520) %u (2**255 - 19) = 0 *)
-      (*   #// cut 0 <=u r01.r0 <u 2**54 * 2**54 + 19 * 2**54 * 2**54 * 4 && *)
-      (*   #//     0 <=u r11.r1 <u 2**54 * 2**54 * 2 + 19 * 2**54 * 2**54 * 3 && *)
-      (*   #//     0 <=u r21.r2 <u 2**54 * 2**54 * 3 + 19 * 2**54 * 2**54 * 2 && *)
-      (*   #//     0 <=u r31.r3 <u 2**54 * 2**54 * 4 + 19 * 2**54 * 2**54 * 1 && *)
-      (*   #//     0 <=u r41.r4 <u 2**54 * 2**54 * 5 *)
       (*  *)
-      (* ################################################################### *)
-      (* # The following should hold at this point: *)
-      (* # *)
-      (* # (x0 + 2^51*x1 + 2^102*x2 + 2^153*x3 + 2^204*x4) * (x0 + 2^51*x1 + 2^102*x2 + 2^153*x3 + 2^204*x4) congruent to (r0h.r0l) + (r1h.r1l)*2^51 + (r2h.r2l)*2^102 + (r3h.r3l)*2^153 + (r4h.r4l)*2^204  [modulo 2^255-19] *)
-      (* #  *)
-      (* # Notation: (X.Y) stands for a 128-bit value with the least significant 64 bits in Y and the 64 most significant bits in X *)
-      (* # *)
-      (* ################################################################### *)
-      (*  *)
-      (*   #// var r0_512 = (r01@u128.r0@u128)@u512 *)
-      (*   #//     r1_512 = (r11@u128.r1@u128)@u512 *)
-      (*   #//     r2_512 = (r21@u128.r2@u128)@u512 *)
-      (*   #//     r3_512 = (r31@u128.r3@u128)@u512 *)
-      (*   #//     r4_512 = (r41@u128.r4@u128)@u512 *)
       (*  *)
       (*   redmask = *[uint64 *] &crypto_sign_ed25519_amd64_51_REDMASK51 *)
-QAssign redmask (QConst crypto_sign_ed25519_amd64_51_REDMASK51);
-      (*    *)
       (*   r01 = (r01.r0) << 13 *)
-QAssign tmp (concat_shift (QVar r01) (QVar r0) (13%positive));
-QSplit r01 tmp (QVar tmp) wsize;
-QSplit tmp r01 (QVar r01) wsize;
       (*   r0 &= redmask *)
-QSplit tmp r0 (QVar r0) crypto_sign_ed25519_amd64_51_REDMASK51_width;
+QSplit tmp r0 (QVar r0) 51%positive;
+QAssign r01 (QBinop QAdd (pow2 (QVar r01) 13%positive) (QVar tmp));
       (*    *)
       (*   r11 = (r11.r1) << 13 *)
-QAssign tmp (concat_shift (QVar r11) (QVar r1) (13%positive));
-QSplit r11 tmp (QVar tmp) wsize;
-QSplit tmp r11 (QVar r11) wsize;
       (*   r1 &= redmask *)
-QSplit tmp r1 (QVar r1) crypto_sign_ed25519_amd64_51_REDMASK51_width;
       (*   r1 += r01 *)
+QSplit tmp r1 (QVar r1) 51%positive;
+QAssign r11 (QBinop QAdd (pow2 (QVar r11) 13%positive) (QVar tmp));
 QAssign r1 (QBinop QAdd (QVar r1) (QVar r01));
       (*    *)
       (*   r21 = (r21.r2) << 13 *)
-QAssign tmp (concat_shift (QVar r21) (QVar r2) (13%positive));
-QSplit r21 tmp (QVar tmp) wsize;
-QSplit tmp r21 (QVar r21) wsize;
       (*   r2 &= redmask *)
-QSplit tmp r2 (QVar r2) crypto_sign_ed25519_amd64_51_REDMASK51_width;
       (*   r2 += r11 *)
+QSplit tmp r2 (QVar r2) 51%positive;
+QAssign r21 (QBinop QAdd (pow2 (QVar r21) 13%positive) (QVar tmp));
 QAssign r2 (QBinop QAdd (QVar r2) (QVar r11));
       (*    *)
       (*   r31 = (r31.r3) << 13 *)
-QAssign tmp (concat_shift (QVar r31) (QVar r3) (13%positive));
-QSplit r31 tmp (QVar tmp) wsize;
-QSplit tmp r31 (QVar r31) wsize;
-       (*   r3 &= redmask *)
-QSplit tmp r3 (QVar r3) wsize;
+      (*   r3 &= redmask *)
       (*   r3 += r21 *)
+QSplit tmp r3 (QVar r3) 51%positive;
+QAssign r31 (QBinop QAdd (pow2 (QVar r31) 13%positive) (QVar tmp));
 QAssign r3 (QBinop QAdd (QVar r3) (QVar r21));
       (*    *)
       (*   r41 = (r41.r4) << 13 *)
-QAssign tmp (concat_shift (QVar r41) (QVar r4) (13%positive));
-QSplit r41 tmp (QVar tmp) wsize;
-QSplit tmp r41 (QVar r41) wsize;
       (*   r4 &= redmask *)
-QSplit tmp r4 (QVar r4) crypto_sign_ed25519_amd64_51_REDMASK51_width;
       (*   r4 += r31 *)
+QSplit tmp r4 (QVar r4) 51%positive;
+QAssign r41 (QBinop QAdd (pow2 (QVar r41) 13%positive) (QVar tmp));
 QAssign r4 (QBinop QAdd (QVar r4) (QVar r31));
       (*   r41 = r41 * 19 *)
 QAssign r41 (QBinop QMul (QVar r41) (QConst 19%Z));
       (*   r0 += r41 *)
 QAssign r0 (QBinop QAdd (QVar r0) (QVar r41));
       (*  *)
-      (*   #// var lhs = r0_512 + r1_512 * 2**51 + r2_512 * 2**102 + r3_512 * 2**153 + r4_512 * 2**204 *)
-      (*   #//     rhs = r0@u512 + r1@u512 * 2**51 + r2@u512 * 2**102 + r3@u512 * 2**153 + r4@u512 * 2**204 *)
-      (*   #// assert lhs >=u rhs && (lhs - rhs) %u (2**255 - 19) = 0 *)
-      (*   #// cut 0 <=u r0 <u 2**64 - 2**63 + 2**62 && *)
-      (*   #//     0 <=u r1 <u 2**64 - 2**63 + 2**61 && *)
-      (*   #//     0 <=u r2 <u 2**63 - 2**60 + 2**59 && *)
-      (*   #//     0 <=u r3 <u 2**62 + 2**61 - 2**59 && *)
-      (*   #//     0 <=u r4 <u 2**61 + 2**60 - 2**56 && *)
-      (*   #//     redmask = mem64[crypto_sign_ed25519_amd64_51_REDMASK51] *)
       (*  *)
-      (*   #// var r0_512 = r0@u512 *)
-      (*   #//     r1_512 = r1@u512 *)
-      (*   #//     r2_512 = r2@u512 *)
-      (*   #//     r3_512 = r3@u512 *)
-      (*   #//     r4_512 = r4@u512 *)
+      (*  *)
       (*  *)
       (*   t = r0 *)
-QAssign t (QVar r0);
       (*   (uint64) t >>= 51 *)
-QSplit t tmp (QVar t) (51%positive);
       (*   t += r1 *)
-QAssign t (QBinop QAdd (QVar t) (QVar r1));
       (*   r0 &= redmask *)
-QSplit tmp r0 (QVar r0) crypto_sign_ed25519_amd64_51_REDMASK51_width;
+QAssign t (QVar r0);
+QSplit t tmp (QVar t) (51%positive);
+QAssign t (QBinop QAdd (QVar t) (QVar r1));
+QAssign r0 (QVar tmp);
       (*    *)
       (*   r1 = t *)
-QAssign r1 (QVar t);
       (*   (uint64) t >>= 51 *)
-QSplit t tmp (QVar t) (51%positive);
       (*   t += r2 *)
-QAssign t (QBinop QAdd (QVar t) (QVar r2));
       (*   r1 &= redmask *)
-QSplit tmp r1 (QVar r1) crypto_sign_ed25519_amd64_51_REDMASK51_width;
+QAssign r1 (QVar t);
+QSplit t tmp (QVar t) (51%positive);
+QAssign t (QBinop QAdd (QVar t) (QVar r2));
+QAssign r1 (QVar tmp);
       (*    *)
       (*   r2 = t *)
-QAssign r2 (QVar t);
       (*   (uint64) t >>= 51 *)
-QSplit t tmp (QVar t) (51%positive);
       (*   t += r3 *)
-QAssign t (QBinop QAdd (QVar t) (QVar r3));
       (*   r2 &= redmask *)
-QSplit tmp r2 (QVar r2) crypto_sign_ed25519_amd64_51_REDMASK51_width;
+QAssign r2 (QVar t);
+QSplit t tmp (QVar t) (51%positive);
+QAssign t (QBinop QAdd (QVar t) (QVar r3));
+QAssign r2 (QVar tmp);
       (*    *)
       (*   r3 = t *)
-QAssign r3 (QVar t);
       (*   (uint64) t >>= 51 *)
-QSplit t tmp (QVar t) (51%positive);
       (*   t += r4 *)
-QAssign t (QBinop QAdd (QVar t) (QVar r4));
       (*   r3 &= redmask *)
-QSplit tmp r3 (QVar r3) crypto_sign_ed25519_amd64_51_REDMASK51_width;
+QAssign r3 (QVar t);
+QSplit t tmp (QVar t) (51%positive);
+QAssign t (QBinop QAdd (QVar t) (QVar r4));
+QAssign r3 (QVar tmp);
       (*    *)
       (*   r4 = t *)
-QAssign r4 (QVar t);
       (*   (uint64) t >>= 51 *)
-QSplit t tmp (QVar t) (51%positive);
       (*   t *= 19 *)
-QAssign t (QBinop QMul (QVar t) (QConst 19%Z));
       (*   r0 += t *)
-QAssign r0 (QBinop QAdd (QVar r0) (QVar t));
       (*   r4 &= redmask *)
-QSplit tmp r4 (QVar r4) crypto_sign_ed25519_amd64_51_REDMASK51_width;
+QAssign r4 (QVar t);
+QSplit t tmp (QVar t) (51%positive);
+QAssign t (QBinop QMul (QVar t) (QConst 19%Z));
+QAssign r0 (QBinop QAdd (QVar r0) (QVar t));
+QAssign r4 (QVar tmp);
       (*   #END MACRO  *)
       (*  *)
-      (*   #// var lhs = r0_512 + r1_512 * 2**51 + r2_512 * 2**102 + r3_512 * 2**153 + r4_512 * 2**204 *)
-      (*   #//     rhs = r0@u512 + r1@u512 * 2**51 + r2@u512 * 2**102 + r3@u512 * 2**153 + r4@u512 * 2**204 *)
-      (*   #// assert lhs >=u rhs && (lhs - rhs) %u (2**255 - 19) = 0 && *)
-      (*   #//        0 <=u r0 <u 2**51 + 2**15 && *)
-      (*   #//        0 <=u r1 <u 2**51 && *)
-      (*   #//        0 <=u r2 <u 2**51 && *)
-      (*   #//        0 <=u r3 <u 2**51 && *)
-      (*   #//        0 <=u r4 <u 2**51 *)
+      (*  *)
+      (*  *)
       (*  *)
       (* *[uint64 *](rp + 0) = r0 *)
 QAssign z0 (QVar r0);
@@ -465,15 +386,6 @@ QAssign z3 (QVar r3);
       (* *[uint64 *](rp + 32) = r4 *)
 QAssign z4 (QVar r4)
       (*   *)
-      (* ################################################################### *)
-      (* # The following should hold at this point: *)
-      (* # *)
-      (* # (x0 + 2^51*x1 + 2^102*x2 + 2^153*x3 + 2^204*x4) * (x0 + 2^51*x1 + 2^102*x2 + 2^153*x3 + 2^204*x4) congruent to (r0l + r1l*2^51 + r2l*2^102 + r3l*2^153 + r4l*2^204)  [modulo 2^255-19] *)
-      (* # *)
-      (* # r0l,r1l,r2l,r3l,r4l are all in [0,2^51+2^15] *)
-      (* # *)
-      (* ################################################################### *)
-      (*    *)
       (*  *)
       (* c1 =c1_stack *)
       (* c2 =c2_stack *)
@@ -485,4 +397,49 @@ QAssign z4 (QVar r4)
       (*  *)
       (* leave *)
 ] .
+
+Definition fe25519_sq_inputs : VS.t :=
+let            x0 :=   0 in
+let            x1 :=   1 in
+let            x2 :=   2 in
+let            x3 :=   3 in
+let            x4 :=   4 in
+VSLemmas.OP.P.of_list [:: x0; x1; x2; x3; x4].
+
+Definition fe25519_sq_pre : bexp := QTrue.
+
+Definition fe25519_sq_post : bexp :=
+let            x0 :=   0 in
+let            x1 :=   1 in
+let            x2 :=   2 in
+let            x3 :=   3 in
+let            x4 :=   4 in
+let            z0 :=   5 in
+let            z1 :=   6 in
+let            z2 :=   7 in
+let            z3 :=   8 in
+let            z4 :=   9 in
+let        n25519 := 57896044618658097711785492504343953926634992332820282019728792003956564819949%positive in
+QEqMod
+  (
+    QPow (radix51 [::QVar x0; QVar x1; QVar x2; QVar x3; QVar x4]) 2
+  )
+  (radix51 [::QVar z0; QVar z1; QVar z2; QVar z3; QVar z4])
+  (n25519).
+
+Definition fe25519_sq_spec :=
+  {| spre := fe25519_sq_pre;
+     sprog := fe25519_sq;
+     spost := fe25519_sq_post |}.
+
+From mathcomp Require Import eqtype ssrbool.
+From mQhasm Require Import Verify.
+
+Lemma valid_fe25519_sq : valid_ispec (fe25519_sq_inputs, fe25519_sq_spec).
+Proof.
+  time "valid_fe25519_sq" verify_ispec.
+Qed.
+
+Close Scope mqhasm_scope.
+Close Scope N_scope.
 
